wip on projecting deltas

src/tls/StreamDeltas.fst
@@ -12,6 +12,7 @@ module S    = StAE
 module MS   = MonotoneSeq
 module C    = Content
 module DS   = DataStream
+module SeqP = FStar.SeqProperties
 
 let deltas i = Seq.seq (DS.delta i) //not yet handling the well-formedness condition of final deltas
 
@@ -32,18 +33,44 @@ let project_one_frag #i = function
 val project_deltas: #i:id -> fs:S.frags i -> Tot (deltas i)
 let project_deltas #i fs = MS.collect project_one_frag fs
 
+val stream_deltas: #i:id -> #rw:rw -> s:StAE.state i rw{authId i} -> HH.t -> GTot (deltas i)
+let stream_deltas #i #rw s h = project_deltas (StAE.fragments s h)
+
+let stream_deltas_snoc (i:id) (frags:StAE.frags i) (f:Content.fragment i)
+  : Lemma (project_deltas (SeqP.snoc frags f) == Seq.append (project_deltas frags) (project_one_frag f))
+  = MS.collect_snoc project_one_frag frags f
+
 //A predicate stating the deltas of s always as ds as a prefix
 let deltas_prefix (#i:id) (#rw:rw) (s:S.state i rw{authId i}) (ds:deltas i) (h:HH.t) 
   : GTot Type0 
   = MS.grows ds (project_deltas (S.fragments s h))
 
-val project_fragment_deltas: #i:id -> #rw:rw -> s:S.state i rw{authId i} -> fs:S.frags i
-		  -> Lemma (requires (MR.witnessed (S.fragments_prefix s fs)))
-		          (ensures (MR.witnessed (deltas_prefix s (project_deltas fs))))
+val project_fragment_deltas: #i:id -> #rw:rw -> s:S.state i rw -> fs:S.frags i
+		  -> Lemma (authId i /\ MR.witnessed (S.fragments_prefix s fs)
+			   ==> MR.witnessed (deltas_prefix s (project_deltas fs)))
+
 let project_fragment_deltas #i #rw s fs =
-  let aux : h:HH.t -> Lemma (S.fragments_prefix s fs h
+  if authId i 
+  then let j : i:id{authId i} = i in
+       let s  : S.state j rw = s in
+       let fs : S.frags j = fs in
+       let aux : h:HH.t -> Lemma (S.fragments_prefix s fs h
 			    ==> deltas_prefix s (project_deltas fs) h) =
 	  fun h -> MS.collect_grows project_one_frag fs (S.fragments s h) in
-  qintro aux;
-  MR.weaken_witness (S.fragments_prefix s fs) (deltas_prefix s (project_deltas fs))
+       let _ = qintro aux in
+       weaken_witness (S.fragments_prefix s fs) (deltas_prefix s (project_deltas fs))
+  else ()
+  
+(*   else () *)
+
+
+(* val project_fragment_deltas: #i:id -> #rw:rw -> s:S.state i rw{authId i} -> fs:S.frags i *)
+(* 		  -> Lemma (requires (MR.witnessed (S.fragments_prefix s fs))) *)
+(* 		          (ensures (MR.witnessed (deltas_prefix s (project_deltas fs)))) *)
+(* let project_fragment_deltas #i #rw s fs = *)
+(*   let aux : h:HH.t -> Lemma (S.fragments_prefix s fs h *)
+(* 			    ==> deltas_prefix s (project_deltas fs) h) = *)
+(* 	  fun h -> MS.collect_grows project_one_frag fs (S.fragments s h) in *)
+(*   qintro aux; *)
+(*   MR.weaken_witness (S.fragments_prefix s fs) (deltas_prefix s (project_deltas fs)) *)
 
